Proved noCreation on the flight

LeanLTLExamples/DistributedSystems/Links.lean
@@ -1,6 +1,8 @@
 import LeanLTL
 import LeanLTLExamples.DistributedSystems.Defs
 
+open Classical
+
 open LeanLTL.Notation
 open LeanLTLExamples.DistributedSystems
 
@@ -11,56 +13,67 @@ instance {α : Type} : Membership α (Option $ Set α) where
   | .some s, a => a ∈ s
   | _, _ => False
 
+theorem mem_imp_some_set {α : Type} x (S : Option $ Set α) (h : x ∈ S) : S.isSome := by
+  match S with
+  | .none => contradiction
+  | .some s => trivial
+
 axiom MaxDeliverTime : ℕ
 
 namespace FairLossLink
   variable {𝓂 : Type}
 
   inductive Request | Send (dest : Process) (msg : 𝓂)
+  -- In distributed system terminology, "deliver" sorta means "receives".
+  -- That's because we are reasoning about the fair-loss link component,
+  -- who will be delivering messages to the process on which it is hosted.
   inductive Indication | Deliver (src : Process) (msg : 𝓂)
 
+  -- Events for a given process.
   structure ε where
     requests : Set $ @Request 𝓂
     indications : Set $ @Indication 𝓂
 
-  -- Events at a point in time for some process
+  -- Events at a point in time for some process.
+  -- If σ p is Option.none for some p, then some p is crashed at that state.
   def σ := Process → Option (@ε 𝓂)
   instance : Inhabited $ @σ 𝓂 where
     default _ := .none
 
-  -- LLTL Version
-  def crashed (s : @σ 𝓂) (p : Process) := (s p).isNone
-  def requests (s : @σ 𝓂) (p : Process) := (s p).map ε.requests
-  def indications (s : @σ 𝓂) (p : Process) := (s p).map ε.indications
-
-  -- Tried to write the most simple one using LLTL and failed.
-  -- def fairLoss' : @ts 𝓂 := LLTL[∀ p₁ p₂ msg,
-  --   (𝐆 (𝐅 ((Request.Send p₂ msg) ∈ ((← requests) p₁))))
-  --     → (𝐆 (𝐅 (crashed ∨ ((Indication.Deliver p₁ msg) ∈ (← indications p₂)))))
-  -- ]
-
-  -- Handmade Version
   def Trace' := Trace $ @σ 𝓂
   def TraceSet' := TraceSet $ @σ 𝓂
+
+  -- Handmade Trace Functions
   def crashedAt (t : @Trace' 𝓂) n (p : Process) := (t.toFun! n p).isNone
   def requestsAt (t : @Trace' 𝓂) n (p : Process) := (t.toFun! n p).map ε.requests
   def indicationsAt (t : @Trace' 𝓂) n (p : Process) := (t.toFun! n p).map ε.indications
 
+  -- LLTL Trace Functions for use in LLTL macro
+  def crashed (s : @σ 𝓂) (p : Process) := (s p).isNone
+  def requests (s : @σ 𝓂) (p : Process) := (s p).map ε.requests
+  def indications (s : @σ 𝓂) (p : Process) := (s p).map ε.indications
+
+  -- If process p₁ sends a message m infinitely often to process p₂,
+  -- then process p₂ will deliver m infinitely often from p₁.
   def fairLoss : @TraceSet' 𝓂 where
     sat t := ∀ (p₁ p₂ : Process) (msg : 𝓂),
       (∀ n, ∃ sendTime, n ≤ sendTime ∧ (.Send p₂ msg) ∈ (requestsAt t sendTime p₁))
-      → (∀ n, ∃ deliverTime, n < deliverTime ∧ (
-          (crashedAt t deliverTime p₂) ∨ (.Deliver p₁ msg) ∈ (indicationsAt t deliverTime p₂)))
+      → (∀ n, ∃ deliverTime > n,
+          (crashedAt t deliverTime p₂) ∨ (.Deliver p₁ msg) ∈ (indicationsAt t deliverTime p₂))
 
+  -- If process p₁ does *not* send a message m infinitely often to process p₂,
+  -- then process p₂ should *not* deliver m infinitely often.
   def finiteDuplication : @TraceSet' 𝓂 where
     sat t := ∀ (p₁ p₂ : Process) (msg : 𝓂),
       (∃ noMoreSending, (.Send p₂ msg) ∉ (requestsAt t noMoreSending p₁))
         → (∃ noMoreDelivering, (.Deliver p₁ msg) ∉ (indicationsAt t noMoreDelivering p₂))
 
+  -- A message does not come out of thin air;
+  -- If process p₂ delivers a message from process p₁,
   def noCreation : @TraceSet' 𝓂 where
     sat t := ∀ (p₁ p₂ : Process) (msg : 𝓂) deliverTime,
       ((.Deliver p₁ msg) ∈ (indicationsAt t deliverTime p₂))
-      → ∃ sendTime, sendTime < deliverTime ∧ deliverTime ≤ sendTime + MaxDeliverTime
+      → ∃ sendTime < deliverTime, deliverTime ≤ sendTime + MaxDeliverTime
           ∧ (.Send p₂ msg) ∈ (requestsAt t sendTime p₁)
 
 end FairLossLink
@@ -81,20 +94,23 @@ namespace StubbornLink
   instance : Inhabited $ @σ 𝓂 where
     default _ := .none
 
-    def T := Trace $ @σ 𝓂
-    def TS := TraceSet $ @σ 𝓂
-    def crashedAt (t : @T 𝓂) n (p : Process) := (t.toFun! n p).isNone
-    def requestsAt (t : @T 𝓂) n (p : Process) := (t.toFun! n p).map ε.requests
-    def indicationsAt (t : @T 𝓂) n (p : Process) := (t.toFun! n p).map ε.indications
+  def Trace' := Trace $ @σ 𝓂
+  def TraceSet' := TraceSet $ @σ 𝓂
 
-    -- LLTL Version
-    def crashed (s : @σ 𝓂) (p : Process) := (s p).isNone
-    def requests (s : @σ 𝓂) (p : Process) := (s p).map ε.requests
-    def indications (s : @σ 𝓂) (p : Process) := (s p).map ε.indications
+  def crashedAt (t : @Trace' 𝓂) n (p : Process) := (t.toFun! n p).isNone
+  def requestsAt (t : @Trace' 𝓂) n (p : Process) := (t.toFun! n p).map ε.requests
+  def indicationsAt (t : @Trace' 𝓂) n (p : Process) := (t.toFun! n p).map ε.indications
+
+  def crashed (s : @σ 𝓂) (p : Process) := (s p).isNone
+  def requests (s : @σ 𝓂) (p : Process) := (s p).map ε.requests
+  def indications (s : @σ 𝓂) (p : Process) := (s p).map ε.indications
 end StubbornLink
-
+-- Unlike the FairLossLink, whose properties are assumed, we write the code for the stubborn link,
+-- and show that it can be made using a fair-loss link.
+--
+-- Afterwards we will reason about its properties.
 open StubbornLink in
-def StubbornLink {𝓂 : Type} : @TS 𝓂 where
+def StubbornLink {𝓂 : Type} : @TraceSet' 𝓂 where
   sat t :=
     -- There is a fair loss link that runs in lockstep with the stubborn link.
     ∃ fll_t : @FairLossLink.Trace' 𝓂, (fll_t ⊨ FairLossLink)
@@ -102,40 +118,44 @@ def StubbornLink {𝓂 : Type} : @TS 𝓂 where
     ∧ fll_t.length = t.length
     -- And a process crashes on both at the same time
     ∧ (∀ n p, crashedAt t n p ↔ FairLossLink.crashedAt fll_t n p)
-    -- Here are the requests made to it.
-    ∧ (∀ n p₁ p₂ msg, ((.Send p₂ msg) ∈ requestsAt t n p₁)
-        → ∀ sendTime, n ≤ sendTime
-        → ((.Send p₂ msg) ∈ FairLossLink.requestsAt fll_t sendTime p₁))
+    -- Here are the only requests made to it.
+    ∧ (∀ n p₁ p₂ msg,
+      (.Send p₂ msg) ∈ (FairLossLink.requestsAt fll_t n p₁)
+        ↔ ∃ sendTime ≤ n, (.Send p₂ msg) ∈ requestsAt t sendTime p₁
+    )
+    -- ∧ (∀ sendTime p₁ p₂ msg, ((.Send p₂ msg) ∈ requestsAt t sendTime p₁)
+    --     ↔ ∀ forwardTime, sendTime ≤ forwardTime
+    --     → ((.Send p₂ msg) ∈ FairLossLink.requestsAt fll_t forwardTime p₁))
     -- Now that we have our fair loss link, and it's up and running, we need to filter our stubborn
     -- link indications.
     -- The stubborn link delivers whenever the fair loss link delivers.
-    ∧ (∀ n p₁ p₂ msg,
-        (.Deliver p₁ msg) ∈ FairLossLink.indicationsAt fll_t n p₂
-        → ((.Deliver p₁ msg) ∈ indicationsAt t n p₂))
+    ∧ (∀ deliverTime p₁ p₂ msg,
+        (.Deliver p₁ msg) ∈ FairLossLink.indicationsAt fll_t deliverTime p₂
+        ↔ ((.Deliver p₁ msg) ∈ indicationsAt t deliverTime p₂))
 
 namespace StubbornLink
   variable {𝓂 : Type}
+  -- Send from p1 to p2 means p2 delivers infinitely often once you've sent it.
   theorem stubbornDelivery (p₁ p₂ : Process) (msg : 𝓂) :
-    -- Send from p1 to p2 means p2 delivers infinitely often once you've sent it.
     ⊨ⁱ LLTL[StubbornLink →
-      𝐆 (𝐅 ((.Send p₂ msg) ∈ ((← requests) p₁))
+      𝐆 (((.Send p₂ msg) ∈ ((← requests) p₁))
       → 𝐆 𝐅 (((← crashed) p₂) = true ∨ (.Deliver p₁ msg) ∈ ((← indications) p₂)))
     ] := by
       simp +contextual [push_ltl]
-      rintro t t_inf ⟨fll_t, ⟨fairloss, fll_t_len, crashes, subreq, delivery⟩⟩ x y req z
+      rintro t t_inf ⟨fll_t, fairloss, fll_t_len, crashes, subreq, delivery⟩ x req z
       unfold FairLossLink at fairloss
       simp +contextual [push_ltl] at fairloss
       replace fairloss := fairloss.1
       unfold FairLossLink.fairLoss at fairloss
       simp at fairloss
       specialize fairloss p₁ p₂ msg
-      have infiniteSend : ∀ (n : ℕ), ∃ sendTime, n ≤ sendTime ∧ FairLossLink.Request.Send p₂ msg ∈ FairLossLink.requestsAt fll_t sendTime p₁ := by
+      -- Suffering
+      have infiniteSend : ∀ (n : ℕ), ∃ sendTime ≥ n, .Send p₂ msg ∈ FairLossLink.requestsAt fll_t sendTime p₁ := by
         intro now
-        specialize subreq (y + x) p₁ p₂ msg
-        unfold requests at req
-        unfold requestsAt at subreq
-        specialize subreq req (now + y + x) (by omega)
-        exists (now + y + x)
+        specialize subreq (now + x) p₁ p₂ msg
+        replace subreq := subreq.mpr
+        specialize subreq ⟨x, by simp, req⟩
+        exists (now + x)
         exact ⟨by omega, subreq⟩
       specialize fairloss infiniteSend (z + x)
       obtain ⟨deliverTime, ⟨deliverTimeLowerBound, crashedOrDelivered⟩⟩ := fairloss
@@ -151,4 +171,37 @@ namespace StubbornLink
         replace delivery := delivery deliverTime p₁ p₂ msg
         unfold indicationsAt at delivery
         unfold indications
-        exact delivery delivered
+        exact delivery.mp delivered
+
+  -- If a message m was stubborn received at time n, it must have been stubborn sent.
+  -- Proof by contradiction:
+  -- 1. Assume m was stubborn received [but was not stubborn sent!]
+  --    Show that this results in a contradiction.
+  --
+  -- 2. m must have been fair-loss received because that's how the stubborn link code works.
+  --
+  -- 3. By the no-creation property on the fair-loss link, m was fair-loss sent at some time n' before n.
+  --
+  -- 4. But we assumed that message m was not stubborn sent before time n!
+  --    Because it was not stubborn sent before time n, then it couldn't have been fair-loss sent before n.
+  --
+  -- Contradiction ∎
+  theorem noCreation (t : Trace') (p₁ p₂ : Process) (msg : 𝓂) deliverTime:
+    (t ⊨ StubbornLink) → ((.Deliver p₁ msg) ∈ (indicationsAt t deliverTime p₂))
+    → ∃ sendTime < deliverTime, (.Send p₂ msg) ∈ (requestsAt t sendTime p₁)
+    := by
+      -- 1.
+      rintro ⟨fll_t, fairloss, sameLength, crashes, sendCode, deliverCode⟩ stubbornDelivery
+      apply byContradiction
+      intro noStubbornSend
+      simp at noStubbornSend
+      -- 2.
+      have fllDelivery := (deliverCode deliverTime p₁ p₂ msg).mpr stubbornDelivery
+      obtain ⟨_, _, noCreation⟩ := fairloss
+      -- 3.
+      replace noCreation := noCreation p₁ p₂ msg deliverTime fllDelivery
+      obtain ⟨n', n'min, n'max, fairlossSend⟩ := noCreation
+      -- TODO: prove no fair loss send
+      obtain ⟨m, mMin, stubbornSend⟩ := (sendCode n' p₁ p₂ msg).mp fairlossSend
+      specialize noStubbornSend m (by omega)
+      contradiction
